Propositional.v
@@ -1,2 +1,2 @@
 (* Here will be theorems about propositional logic.
-THen I'll decide how to unite it with the rest. *)
+Then I'll decide how to unite it with the rest. *)
